# HW5

## 2

1. $$1 - \frac{M-m}{M} \cdot \frac{M-m-1}{M-1}= \frac{2mM - m^2 - m}{M(M-1)}$$

2. $$\frac{{{m} \choose {2}}}{{m \choose 2} + {m \choose 1} \cdot {M - m \choose 1}} = \frac{m - 1}{2M - m -1}$$

3. $$\frac{{m \choose 1}\cdot {M - m \choose 1}}{{M - m \choose 2} + {M -m \choose 1} \cdot {m \choose 1}} = \frac{2m}{M - m + 1}$$

## 4

定义:

$$
f_k = \sum_{i=k}^{+\infty} \alpha p^i \cdot \frac{{i \choose k}}{2^i}
$$

所求为 $f_k$. 令 $\beta = \frac{p}{2}$. 即为:

$$
\begin{aligned}
f_k
&= \alpha \beta ^ k \sum_{i=0}^{+\infty} \beta^i \cdot {k + i \choose k} \\
&= \alpha \beta ^ k (1 - \beta) ^ {-k - 1} (\text{广义二项式展开}) \\
&= \alpha p ^ k (2 - p) ^ {-k - 1}
\end{aligned}
$$

## 7

$$
\frac{0.1 \cdot 0.05}{0.1 \cdot 0.05 + 0.7 \cdot 0.1 + 0.2 \cdot 0.2} = \frac {1} {23}
$$

## 9

$$
\frac{1 * 0.5}{0.25 * 0.5 + 1 * 0.5} = 0.8
$$

## 11

$$
\begin{aligned}
    & p_1 \sum_{k = 0}^{\infty}{((1 - p_1)(1 - p_2)) ^ k} \\
=~\ & \frac{p_1}{p_1 + p_2 - p_1 p_2}
\end{aligned}
$$

## 12

$$ 0.1 * 1 + (1 - 0.1) * 0.1 + 0.2 * 0.2 = 0.23 $$
